concurrency/scache/CacheInit.i.dfy
@@ -21,6 +21,7 @@ module CacheInit(aio: AIO(CacheAIOParams, CacheIfc, CacheSSM)) {
   import opened CacheResources
   import opened GlinearOption
   import opened CacheAIOParams
+  import CacheSSM
   import opened BasicLockImpl
   import opened MemSplit
   import opened GhostLoc
@@ -29,18 +30,19 @@ module CacheInit(aio: AIO(CacheAIOParams, CacheIfc, CacheSSM)) {
   import RwLock
   import opened PageSizeConstant
 
-  method init_batch_busy()
+  method init_batch_busy(config: Config)
   returns (linear batch_busy: lseq<Atomic<bool, NullGhostType>>)
-  ensures |batch_busy| == NUM_CHUNKS as int
-  ensures (forall i :: 0 <= i < NUM_CHUNKS as int ==> lseq_has(batch_busy)[i])
-  ensures (forall i, v, g :: 0 <= i < NUM_CHUNKS as int ==> atomic_inv(batch_busy[i], v, g) <==> true)
+  requires config.WF()
+  ensures |batch_busy| == config.batch_capacity as int
+  ensures (forall i :: 0 <= i < config.batch_capacity as int ==> lseq_has(batch_busy)[i])
+  ensures (forall i, v, g :: 0 <= i < config.batch_capacity as int ==> atomic_inv(batch_busy[i], v, g) <==> true)
   {
-    batch_busy := lseq_alloc<Atomic<bool, NullGhostType>>(NUM_CHUNKS_64());
+    batch_busy := lseq_alloc<Atomic<bool, NullGhostType>>(config.batch_capacity);
     var i: uint64 := 0;
-    while i < NUM_CHUNKS_64()
-    invariant 0 <= i as int <= NUM_CHUNKS as int
-    invariant |batch_busy| == NUM_CHUNKS as int
-    invariant (forall j :: i as int <= j < NUM_CHUNKS as int ==> !lseq_has(batch_busy)[j])
+    while i < config.batch_capacity
+    invariant 0 <= i as int <= config.batch_capacity as int
+    invariant |batch_busy| == config.batch_capacity as int
+    invariant (forall j :: i as int <= j < config.batch_capacity as int ==> !lseq_has(batch_busy)[j])
     invariant (forall j :: 0 <= j < i as int ==> lseq_has(batch_busy)[j])
     invariant (forall j, v, g :: 0 <= j < i as int ==> atomic_inv(batch_busy[j], v, g) <==> true)
     {
@@ -50,11 +52,12 @@ module CacheInit(aio: AIO(CacheAIOParams, CacheIfc, CacheSSM)) {
     }
   }
 
-  method init_ioslots()
+  method init_ioslots(config: Config)
   returns (iocb_base_ptr: Ptr, linear io_slots: lseq<IOSlot>)
+  requires config.WF()
   ensures |io_slots| == NUM_IO_SLOTS as int
   ensures (forall i | 0 <= i < |io_slots| :: lseq_has(io_slots)[i])
-  ensures (forall i | 0 <= i < |io_slots| :: io_slots[i].WF())
+  ensures (forall i | 0 <= i < |io_slots| :: io_slots[i].WF(config))
   ensures (forall i | 0 <= i < |io_slots| ::
           iocb_base_ptr.as_nat() + i * SizeOfIocb() as int < 0x1_0000_0000_0000_0000
           && 0 <= i * SizeOfIocb() as int < 0x1_0000_0000_0000_0000
@@ -70,8 +73,8 @@ module CacheInit(aio: AIO(CacheAIOParams, CacheIfc, CacheSSM)) {
     var full_iovec_ptr;
     glinear var full_iovec;
     var dummy_iovec := new_iovec(nullptr(), 0);
-    full_iovec_ptr, full_iovec := alloc_array(PAGES_PER_EXTENT_64() * NUM_IO_SLOTS_64(), dummy_iovec);
-    glinear var iovecs := mem_split(full_iovec, PAGES_PER_EXTENT, NUM_IO_SLOTS);
+    full_iovec_ptr, full_iovec := alloc_array(config.pages_per_extent * NUM_IO_SLOTS_64(), dummy_iovec);
+    glinear var iovecs := mem_split(full_iovec, config.pages_per_extent as int, NUM_IO_SLOTS);
 
     ghost var iocbs_copy := iocbs;
 
@@ -83,27 +86,30 @@ module CacheInit(aio: AIO(CacheAIOParams, CacheIfc, CacheSSM)) {
     invariant |io_slots| == NUM_IO_SLOTS as int
     invariant forall j | i3 as int <= j < NUM_IO_SLOTS as int :: j !in io_slots
     invariant forall j | 0 <= j < i3 as int :: j in io_slots
-        && io_slots[j].WF()
+        && io_slots[j].WF(config)
         && iocb_base_ptr.as_nat() + j * SizeOfIocb() as int < 0x1_0000_0000_0000_0000
         && 0 <= j * SizeOfIocb() as int < 0x1_0000_0000_0000_0000
         && io_slots[j].iocb_ptr == ptr_add(iocb_base_ptr, j as uint64 * SizeOfIocb())
     invariant forall j | i3 as int <= j < NUM_IO_SLOTS as int ::
-        has_single(full_iovec, PAGES_PER_EXTENT, iovecs, j)
+        has_single(full_iovec, config.pages_per_extent as int, iovecs, j)
     {
       ghost var old_iovecs := iovecs;
 
       glinear var iocb;
       iocbs, iocb := glmap_take(iocbs, i3 as int);
 
-      assert has_single(full_iovec, PAGES_PER_EXTENT, iovecs, i3 as int);
+      assert has_single(full_iovec, config.pages_per_extent as int, iovecs, i3 as int);
       assert (i3 as int) in iovecs;
-      NonlinearLemmas.mul_ge_0(i3 as int, sizeof<Iovec>() as int);
-      var iovec_ptr := ptr_add(full_iovec_ptr, i3 * PAGES_PER_EXTENT_64() * sizeof<Iovec>());
+      NonlinearLemmas.mul_ge_0(i3 as int, config.pages_per_extent as int);
+      NonlinearLemmas.mul_ge_0(i3 as int * config.pages_per_extent as int, sizeof<Iovec>() as int);
+      NonlinearLemmas.mul_le_right(i3 as int, config.pages_per_extent as int, 0x1_0000);
+          
+      var iovec_ptr := ptr_add(full_iovec_ptr, i3 * config.pages_per_extent * sizeof<Iovec>());
       glinear var iovec;
       iovecs, iovec := glmap_take(iovecs, i3 as int);
 
       assert iovec.ptr == iovec_ptr;
-      assert |iovec.s| == PAGES_PER_EXTENT as int;
+      assert |iovec.s| == config.pages_per_extent as int;
 
       glinear var io_slot_access := IOSlotAccess(iocb, iovec);
 
@@ -112,35 +118,38 @@ module CacheInit(aio: AIO(CacheAIOParams, CacheIfc, CacheSSM)) {
         (slot_access: IOSlotAccess) =>
           && slot_access.iocb.ptr == iocb_ptr
           && slot_access.iovec.ptr == iovec_ptr
-          && |slot_access.iovec.s| == PAGES_PER_EXTENT as int
+          && |slot_access.iovec.s| == config.pages_per_extent as int
       );
       linear var io_slot := IOSlot(
           iocb_ptr,
           iovec_ptr,
           slot_lock);
-      assert io_slot.WF();
+      assert io_slot.WF(config);
       lseq_give_inout(inout io_slots, i3, io_slot);
 
       i3 := i3 + 1;
 
       assert forall j | i3 as int <= j < NUM_IO_SLOTS as int ::
-          has_single(full_iovec, PAGES_PER_EXTENT, old_iovecs, j) ==>
-          has_single(full_iovec, PAGES_PER_EXTENT, iovecs, j);
+          has_single(full_iovec, config.pages_per_extent as int, old_iovecs, j) ==>
+          has_single(full_iovec, config.pages_per_extent as int, iovecs, j);
     }
 
     dispose_anything(iocbs);
     dispose_anything(iovecs);
   }
 
-  predicate {:opaque} refcount_i_inv(read_refcounts_array: lseq<AtomicRefcount>,
+  predicate {:opaque} refcount_i_inv(
+        config: Config,
+        read_refcounts_array: lseq<AtomicRefcount>,
         status_idx_array: lseq<StatusIdx>,
         counter_loc: Loc,
         i': int, j': int)
-  requires |status_idx_array| == CACHE_SIZE as int
-  requires |read_refcounts_array| == RC_WIDTH as int * CACHE_SIZE as int
-  requires 0 <= i' < CACHE_SIZE as int && 0 <= j' < RC_WIDTH as int
+  requires config.WF()
+  requires |status_idx_array| == config.cache_size as int
+  requires |read_refcounts_array| == RC_WIDTH as int * config.cache_size as int
+  requires 0 <= i' < config.cache_size as int && 0 <= j' < RC_WIDTH as int
   {
-    && var rci := rc_index(j' as uint64, i' as uint32) as int;
+    && var rci := rc_index(config, j' as uint64, i' as uint32) as int;
     && rci in read_refcounts_array
     && read_refcounts_array[rci].inv(j')
     && read_refcounts_array[rci].rwlock_loc
@@ -153,168 +162,152 @@ module CacheInit(aio: AIO(CacheAIOParams, CacheIfc, CacheSSM)) {
   // use this trigger as a workaround
   predicate True(a: nat, b: nat) { true }
 
-  predicate refcount_i_inv_i(read_refcounts_array: lseq<AtomicRefcount>,
+  predicate refcount_i_inv_i(
+        config: Config,
+        read_refcounts_array: lseq<AtomicRefcount>,
         status_idx_array: lseq<StatusIdx>,
         counter_loc: Loc,
         i: int)
-  requires |status_idx_array| == CACHE_SIZE as int
-  requires |read_refcounts_array| == RC_WIDTH as int * CACHE_SIZE as int
-  requires 0 <= i <= CACHE_SIZE as int
+  requires config.WF()
+  requires |status_idx_array| == config.cache_size as int
+  requires |read_refcounts_array| == RC_WIDTH as int * config.cache_size as int
+  requires 0 <= i <= config.cache_size as int
   {
     && (forall i', j' {:trigger True(i',j')} |
           (0 <= i' < i as int && 0 <= j' < RC_WIDTH as int) ::
-        refcount_i_inv(read_refcounts_array, status_idx_array, counter_loc, i', j'))
+        refcount_i_inv(config, read_refcounts_array, status_idx_array, counter_loc, i', j'))
   }
 
-  predicate refcount_i_inv_ij(read_refcounts_array: lseq<AtomicRefcount>,
+  predicate refcount_i_inv_ij(
+        config: Config,
+        read_refcounts_array: lseq<AtomicRefcount>,
         status_idx_array: lseq<StatusIdx>,
         counter_loc: Loc,
         i: int, j: int)
-  requires |status_idx_array| == CACHE_SIZE as int
-  requires |read_refcounts_array| == RC_WIDTH as int * CACHE_SIZE as int
-  requires 0 <= i < CACHE_SIZE as int && 0 <= j <= RC_WIDTH as int
+  requires config.WF()
+  requires |status_idx_array| == config.cache_size as int
+  requires |read_refcounts_array| == RC_WIDTH as int * config.cache_size as int
+  requires 0 <= i < config.cache_size as int && 0 <= j <= RC_WIDTH as int
   {
     && (forall i', j' {:trigger True(i',j')} |
           (0 <= i' < i as int && 0 <= j' < RC_WIDTH as int) ::
-        refcount_i_inv(read_refcounts_array, status_idx_array, counter_loc, i', j'))
+        refcount_i_inv(config, read_refcounts_array, status_idx_array, counter_loc, i', j'))
     && (forall j': int {:Trigger True(i,j')} |
           (0 <= j' < j as int) ::
-        refcount_i_inv(read_refcounts_array, status_idx_array, counter_loc, i, j'))
+        refcount_i_inv(config, read_refcounts_array, status_idx_array, counter_loc, i, j'))
   }
 
-  lemma refcount_i_inv_ij_base(read_refcounts_array: lseq<AtomicRefcount>,
+  lemma refcount_i_inv_ij_base(
+        config: Config,
+        read_refcounts_array: lseq<AtomicRefcount>,
         status_idx_array: lseq<StatusIdx>,
         status_idx_array': lseq<StatusIdx>,
         counter_loc: Loc,
         i: int)
-  requires |status_idx_array'| == |status_idx_array| == CACHE_SIZE as int
-  requires |read_refcounts_array| == RC_WIDTH as int * CACHE_SIZE as int
-  requires 0 <= i < CACHE_SIZE
+  requires config.WF()
+  requires |status_idx_array'| == |status_idx_array| == config.cache_size as int
+  requires |read_refcounts_array| == RC_WIDTH as int * config.cache_size as int
+  requires 0 <= i < config.cache_size as int
   requires forall k | 0 <= k < i :: k in status_idx_array && k in status_idx_array'
       && status_idx_array[k] == status_idx_array'[k]
-  requires refcount_i_inv_i(read_refcounts_array, status_idx_array, counter_loc, i)
-  ensures refcount_i_inv_ij(read_refcounts_array, status_idx_array', counter_loc, i, 0)
+  requires refcount_i_inv_i(config, read_refcounts_array, status_idx_array, counter_loc, i)
+  ensures refcount_i_inv_ij(config, read_refcounts_array, status_idx_array', counter_loc, i, 0)
   {
     forall i', j' | (0 <= i' < i as int && 0 <= j' < RC_WIDTH as int)
-    ensures refcount_i_inv(read_refcounts_array, status_idx_array', counter_loc, i', j');
+    ensures refcount_i_inv(config, read_refcounts_array, status_idx_array', counter_loc, i', j');
     {
       assert True(i', j');
-      assert refcount_i_inv(read_refcounts_array, status_idx_array, counter_loc, i', j');
+      assert refcount_i_inv(config, read_refcounts_array, status_idx_array, counter_loc, i', j');
       reveal_refcount_i_inv();
     }
   }
 
   lemma refcount_i_inv_ij_inc(
+        config: Config,
         read_refcounts_array: lseq<AtomicRefcount>,
         read_refcounts_array': lseq<AtomicRefcount>,
         status_idx_array: lseq<StatusIdx>,
         counter_loc: Loc,
         i: int, j: int)
-  requires 0 <= i < CACHE_SIZE as int && 0 <= j < RC_WIDTH as int
-  requires |status_idx_array| == CACHE_SIZE as int
-  requires |read_refcounts_array| == |read_refcounts_array'| == RC_WIDTH * CACHE_SIZE
+  requires config.WF()
+  requires 0 <= i < config.cache_size as int && 0 <= j < RC_WIDTH as int
+  requires |status_idx_array| == config.cache_size as int
+  requires |read_refcounts_array| == |read_refcounts_array'| == RC_WIDTH * config.cache_size as int
   requires forall k | 0 <= k < |read_refcounts_array| && k in read_refcounts_array
       :: k in read_refcounts_array' && read_refcounts_array'[k] == read_refcounts_array[k]
-  requires refcount_i_inv_ij(read_refcounts_array, status_idx_array, counter_loc, i, j)
-  requires refcount_i_inv(read_refcounts_array', status_idx_array, counter_loc, i, j)
-  ensures refcount_i_inv_ij(read_refcounts_array', status_idx_array, counter_loc, i, j + 1)
+  requires refcount_i_inv_ij(config, read_refcounts_array, status_idx_array, counter_loc, i, j)
+  requires refcount_i_inv(config, read_refcounts_array', status_idx_array, counter_loc, i, j)
+  ensures refcount_i_inv_ij(config, read_refcounts_array', status_idx_array, counter_loc, i, j + 1)
   {
     forall i', j' | (0 <= i' < i as int && 0 <= j' < RC_WIDTH as int)
-    ensures refcount_i_inv(read_refcounts_array', status_idx_array, counter_loc, i', j')
+    ensures refcount_i_inv(config, read_refcounts_array', status_idx_array, counter_loc, i', j')
     {
       assert True(i', j');
-      assert refcount_i_inv(read_refcounts_array, status_idx_array, counter_loc, i', j');
+      assert refcount_i_inv(config, read_refcounts_array, status_idx_array, counter_loc, i', j');
       reveal_refcount_i_inv();
     }
     forall j': int | (0 <= j' < j as int + 1)
-    ensures refcount_i_inv(read_refcounts_array', status_idx_array, counter_loc, i, j')
+    ensures refcount_i_inv(config, read_refcounts_array', status_idx_array, counter_loc, i, j')
     {
       if j' == j {
-        assert refcount_i_inv(read_refcounts_array', status_idx_array, counter_loc, i, j');
+        assert refcount_i_inv(config, read_refcounts_array', status_idx_array, counter_loc, i, j');
       } else {
         assert True(i, j');
-        assert refcount_i_inv(read_refcounts_array, status_idx_array, counter_loc, i, j');
+        assert refcount_i_inv(config, read_refcounts_array, status_idx_array, counter_loc, i, j');
         reveal_refcount_i_inv();
-        assert refcount_i_inv(read_refcounts_array', status_idx_array, counter_loc, i, j');
+        assert refcount_i_inv(config, read_refcounts_array', status_idx_array, counter_loc, i, j');
       }
     }
   }
 
-  lemma refcount_i_inv_ij_end(read_refcounts_array: lseq<AtomicRefcount>,
+  lemma refcount_i_inv_ij_end(
+        config: Config,
+        read_refcounts_array: lseq<AtomicRefcount>,
         status_idx_array: lseq<StatusIdx>,
         counter_loc: Loc,
         i: int)
-  requires |status_idx_array| == CACHE_SIZE
-  requires |read_refcounts_array| == RC_WIDTH * CACHE_SIZE
-  requires 0 <= i < CACHE_SIZE
-  requires refcount_i_inv_ij(read_refcounts_array, status_idx_array, counter_loc, i, RC_WIDTH)
-  ensures refcount_i_inv_i(read_refcounts_array, status_idx_array, counter_loc, i+1)
+  requires config.WF()
+  requires |status_idx_array| == config.cache_size as int
+  requires |read_refcounts_array| == RC_WIDTH * config.cache_size as int
+  requires 0 <= i < config.cache_size as int
+  requires refcount_i_inv_ij(config, read_refcounts_array, status_idx_array, counter_loc, i, RC_WIDTH)
+  ensures refcount_i_inv_i(config, read_refcounts_array, status_idx_array, counter_loc, i+1)
   {
     forall i', j' | (0 <= i' < i + 1 && 0 <= j' < RC_WIDTH)
-    ensures refcount_i_inv(read_refcounts_array, status_idx_array, counter_loc, i', j')
+    ensures refcount_i_inv(config, read_refcounts_array, status_idx_array, counter_loc, i', j')
     {
       assert True(i', j');
     }
   }
 
   lemma refcount_i_inv_i_get(
+      config: Config,
       read_refcounts_array: lseq<AtomicRefcount>,
       status_idx_array: lseq<StatusIdx>,
         counter_loc: Loc,
       i: nat, i': nat, j': nat)
-  requires |status_idx_array| == CACHE_SIZE as int
-  requires |read_refcounts_array| == RC_WIDTH as int * CACHE_SIZE as int
-  requires 0 <= i <= CACHE_SIZE as int
-  requires refcount_i_inv_i(read_refcounts_array, status_idx_array, counter_loc, i)
+  requires config.WF()
+  requires |status_idx_array| == config.cache_size as int
+  requires |read_refcounts_array| == RC_WIDTH as int * config.cache_size as int
+  requires 0 <= i <= config.cache_size as int
+  requires refcount_i_inv_i(config, read_refcounts_array, status_idx_array, counter_loc, i)
   requires 0 <= i' < i
   requires 0 <= j' < RC_WIDTH
-  ensures refcount_i_inv(read_refcounts_array, status_idx_array, counter_loc, i', j')
+  ensures refcount_i_inv(config, read_refcounts_array, status_idx_array, counter_loc, i', j')
   {
     assert True(i', j');
-    assert refcount_i_inv(read_refcounts_array, status_idx_array, counter_loc, i', j');
+    assert refcount_i_inv(config, read_refcounts_array, status_idx_array, counter_loc, i', j');
   }
 
-  lemma inverse_rc_index(k: int)
-  returns (j: int, i: int)
-  requires 0 <= k as int < RC_WIDTH as int * CACHE_SIZE as int
-  ensures 0 <= j as int < RC_WIDTH as int
-  ensures 0 <= i as int < CACHE_SIZE as int
-  ensures k == rc_index(j as uint64, i as uint32) as int
-  {
-    j := k / CACHE_SIZE;
-    var rc_number := k % CACHE_SIZE;
-
-    var cacheline_capacity: int := (CACHE_SIZE_64() / PLATFORM_CACHELINE_SIZE_64()) as int;
-    assert cacheline_capacity as int == CACHELINE_CAPACITY();
-
-    i := (rc_number % (PLATFORM_CACHELINE_SIZE_64() as int)) * cacheline_capacity
-        + (rc_number / (PLATFORM_CACHELINE_SIZE_64() as int));
-
-    var rc_number2 := (i % cacheline_capacity) * (PLATFORM_CACHELINE_SIZE_64() as int)
-        + (i / cacheline_capacity);
-
-    calc {
-      rc_number2 % (PLATFORM_CACHELINE_SIZE_64() as int);
-      (i / cacheline_capacity);
-      rc_number % (PLATFORM_CACHELINE_SIZE_64() as int);
-    }
-
-    calc {
-      rc_number2 / (PLATFORM_CACHELINE_SIZE_64() as int);
-      (i % cacheline_capacity);
-      rc_number / (PLATFORM_CACHELINE_SIZE_64() as int);
-    }
-
-    assert rc_number == rc_number2;
-    reveal_rc_index();
-  }
-
-  method init_cache(glinear init_tok: T.Token)
+  method init_cache(glinear init_tok: T.Token, preConfig: PreConfig)
   returns (linear c: Cache, glinear counter: Clients)
   requires CacheSSM.Init(init_tok.val)
+  requires preConfig.WF()
   ensures c.Inv()
   ensures counter.loc == c.counter_loc && counter.n == 255
   {
+    var config := fromPreConfig(preConfig);
+
     counter := counter_init();
     ghost var counter_loc := counter.loc;
 
@@ -322,44 +315,45 @@ module CacheInit(aio: AIO(CacheAIOParams, CacheIfc, CacheSSM)) {
     glinear var data_pta_full;
     sizeof_int_types();
     data_base_ptr, data_pta_full := alloc_array_hugetables<byte>(
-        CACHE_SIZE_64() * PageSize64(), 0);
+        config.cache_size as uint64 * PageSize64(), 0);
     glinear var data_pta_seq : map<nat, PointsToArray<byte>> :=
-        mem_split(data_pta_full, PageSize as int, CACHE_SIZE);
+        mem_split(data_pta_full, PageSize as int, config.cache_size as int);
 
-    linear var read_refcounts_array := lseq_alloc_hugetables<AtomicRefcount>(RC_WIDTH_64() * CACHE_SIZE_64());
-    linear var status_idx_array := lseq_alloc<StatusIdx>(CACHE_SIZE_64());
+    linear var read_refcounts_array := lseq_alloc_hugetables<AtomicRefcount>(RC_WIDTH_64() * config.cache_size as uint64);
+    linear var status_idx_array := lseq_alloc<StatusIdx>(config.cache_size as uint64);
 
     glinear var dis, empty_seq := split_init(init_tok);
 
-    forall i | 0 <= i < CACHE_SIZE
+    forall i | 0 <= i < config.cache_size as int
     ensures i in data_pta_seq
     {
       assert has_single(data_pta_full, PageSize as int, data_pta_seq, i);
     }
 
-    ghost var data := seq(CACHE_SIZE as int, (i) requires 0 <= i < CACHE_SIZE as int =>
+    ghost var data := seq(config.cache_size as int, (i) requires 0 <= i < config.cache_size as int =>
         data_pta_seq[i].ptr);
 
     ghost var data_pta_seq_copy := data_pta_seq;
 
     var i: uint64 := 0;
-    while i < CACHE_SIZE_64()
-    invariant 0 <= i as int <= CACHE_SIZE as int
-    invariant empty_seq == EmptySeq(i as nat, CACHE_SIZE as int)
-    invariant forall j | i as int <= j < CACHE_SIZE as int :: 
+    while i < config.cache_size as uint64
+    invariant 0 <= i as int <= config.cache_size as int
+    invariant empty_seq == EmptySeq(i as nat, CacheSSM.MAX_CACHE_SIZE)
+    invariant forall j | i as int <= j < config.cache_size as int :: 
         j in data_pta_seq && data_pta_seq[j] == data_pta_seq_copy[j]
-    invariant |status_idx_array| == CACHE_SIZE as int
-    invariant forall j | i as int <= j < CACHE_SIZE as int :: j !in status_idx_array
+    invariant |status_idx_array| == config.cache_size as int
+    invariant forall j | i as int <= j < config.cache_size as int :: j !in status_idx_array
     invariant forall j | 0 <= j < i as int :: j in status_idx_array
         && status_idx_array[j].status.inv()
+        && status_idx_array[j].status.config == config
         && status_idx_array[j].status.key == Key(data[j], status_idx_array[j].page_handle, j)
 
-    invariant |read_refcounts_array| == RC_WIDTH as int * CACHE_SIZE as int
-    invariant forall i', j' | i as int <= i' < CACHE_SIZE as int && 0 <= j' < RC_WIDTH as int ::
-        (rc_index(j' as uint64, i' as uint32) as int) !in read_refcounts_array
-    invariant refcount_i_inv_i(read_refcounts_array, status_idx_array, counter_loc, i as int)
+    invariant |read_refcounts_array| == RC_WIDTH as int * config.cache_size as int
+    invariant forall i', j' | i as int <= i' < config.cache_size as int && 0 <= j' < RC_WIDTH as int ::
+        (rc_index(config, j' as uint64, i' as uint32) as int) !in read_refcounts_array
+    invariant refcount_i_inv_i(config, read_refcounts_array, status_idx_array, counter_loc, i as int)
 
-    decreases CACHE_SIZE as int - i as int
+    decreases config.cache_size as int - i as int
     {
       linear var cell_idx;
       glinear var cell_idx_contents;
@@ -382,43 +376,43 @@ module CacheInit(aio: AIO(CacheAIOParams, CacheIfc, CacheSSM)) {
       ghost var key := Key(data_pta.ptr, cell_idx, i as nat);
 
       glinear var cache_empty;
-      cache_empty, empty_seq := pop_EmptySeq(empty_seq, i as nat, CACHE_SIZE as int);
+      cache_empty, empty_seq := pop_EmptySeq(empty_seq, i as nat, CacheSSM.MAX_CACHE_SIZE);
       glinear var handle := CacheEmptyHandle(key, cache_empty, cell_idx_contents, data_pta);
       glinear var central, rcs := RwLockToken.perform_Init(handle);
       ghost var rwlock_loc := central.loc;
 
       assert AtomicStatusImpl.state_inv(flag_unmapped(), 
           AtomicStatusImpl.G(central, glNone),
-          key, rwlock_loc);
+          key, config, rwlock_loc);
       linear var atomic_status_atomic := new_atomic(
           flag_unmapped(),
           AtomicStatusImpl.G(central, glNone),
-          (v, g) => AtomicStatusImpl.state_inv(v, g, key, rwlock_loc),
+          (v, g) => AtomicStatusImpl.state_inv(v, g, key, config, rwlock_loc),
           0);
       linear var atomic_status := AtomicStatus(
           atomic_status_atomic,
           rwlock_loc,
-          key);
+          key, config);
 
       linear var status_idx := StatusIdx(atomic_status, cell_idx);
       ghost var sia := status_idx_array;
       lseq_give_inout(inout status_idx_array, i, status_idx);
 
-      refcount_i_inv_ij_base(read_refcounts_array, sia, status_idx_array, counter_loc, i as int);
+      refcount_i_inv_ij_base(config, read_refcounts_array, sia, status_idx_array, counter_loc, i as int);
 
       var j : uint64 := 0;
       while j < RC_WIDTH_64()
-      invariant 0 <= i as int < CACHE_SIZE as int
+      invariant 0 <= i as int < config.cache_size as int
       invariant 0 <= j as int <= RC_WIDTH as int
       invariant rcs.val == RwLock.Rcs(j as nat, RC_WIDTH as int)
       invariant rcs.loc == rwlock_loc
 
-      invariant |read_refcounts_array| == RC_WIDTH as int * CACHE_SIZE as int
-      invariant forall i', j' | i as int < i' < CACHE_SIZE as int && 0 <= j' < RC_WIDTH as int ::
-          rc_index(j' as uint64, i' as uint32) as int !in read_refcounts_array
+      invariant |read_refcounts_array| == RC_WIDTH as int * config.cache_size as int
+      invariant forall i', j' | i as int < i' < config.cache_size as int && 0 <= j' < RC_WIDTH as int ::
+          rc_index(config, j' as uint64, i' as uint32) as int !in read_refcounts_array
       invariant forall j' | j as int <= j' < RC_WIDTH as int ::
-          rc_index(j' as uint64, i as uint32) as int !in read_refcounts_array
-      invariant refcount_i_inv_ij(read_refcounts_array, status_idx_array, counter_loc, i as int, j as int)
+          rc_index(config, j' as uint64, i as uint32) as int !in read_refcounts_array
+      invariant refcount_i_inv_ij(config, read_refcounts_array, status_idx_array, counter_loc, i as int, j as int)
 
       decreases RC_WIDTH as int - j as int
       {
@@ -435,36 +429,31 @@ module CacheInit(aio: AIO(CacheAIOParams, CacheIfc, CacheSSM)) {
 
         // XXX I don't care about the perf of the initialization method, but do note
         // that the access pattern for writing to this array might be completely awful.
-        lseq_give_inout(inout read_refcounts_array, rc_index(j, i as uint32), ar);
+        lseq_give_inout(inout read_refcounts_array, rc_index(config, j, i as uint32), ar);
 
-        assert refcount_i_inv(read_refcounts_array, status_idx_array, counter_loc, i as int, j as int) by {
+        assert refcount_i_inv(config, read_refcounts_array, status_idx_array, counter_loc, i as int, j as int) by {
           reveal_refcount_i_inv();
         }
 
-        refcount_i_inv_ij_inc(rra, read_refcounts_array, status_idx_array, counter_loc, i as int, j as int);
+        refcount_i_inv_ij_inc(config, rra, read_refcounts_array, status_idx_array, counter_loc, i as int, j as int);
 
         j := j + 1;
 
-        forall i', j' | i as int < i' < CACHE_SIZE as int && 0 <= j' < RC_WIDTH as int
+        forall i', j' | i as int < i' < config.cache_size as int && 0 <= j' < RC_WIDTH as int
         //ensures rc_index(j' as uint64, i' as uint64) as int !in read_refcounts_array
-        ensures rc_index(j' as uint64, i' as uint32) != rc_index(j-1, i as uint32)
+        ensures rc_index(config, j' as uint64, i' as uint32) != rc_index(config, j-1, i as uint32)
         {
-          reveal_rc_index();
-          var cacheline_capacity := CACHE_SIZE_64() / PLATFORM_CACHELINE_SIZE_64();
-          assert cacheline_capacity as int == CACHELINE_CAPACITY();
-          assert rc_index(j' as uint64, i' as uint32) != rc_index(j-1, i as uint32);
+          rc_index_inj(config, j', i', j as int - 1, i as int);
         }
-        /*
         forall j' | j as int <= j' < RC_WIDTH as int
-        ensures rc_index(j' as uint64, i as uint64) as int !in read_refcounts_array
+        ensures rc_index(config, j' as uint64, i as uint32) as int !in read_refcounts_array
         {
-          reveal_rc_index();
+          rc_index_inj(config, j', i as int, j as int - 1, i as int);
         }
-        */
         reveal_rc_index();
       }
 
-      refcount_i_inv_ij_end(read_refcounts_array, status_idx_array, counter_loc, i as int);
+      refcount_i_inv_ij_end(config, read_refcounts_array, status_idx_array, counter_loc, i as int);
       dispose_anything(rcs);
 
       i := i + 1;
@@ -472,22 +461,22 @@ module CacheInit(aio: AIO(CacheAIOParams, CacheIfc, CacheSSM)) {
 
     assert {:split_here} true;
 
-    linear var cache_idx_of_page_array := lseq_alloc(NUM_DISK_PAGES_64());
+    linear var cache_idx_of_page_array := lseq_alloc(config.num_disk_pages);
 
     var i2 := 0;
-    while i2 < NUM_DISK_PAGES_64()
-    invariant 0 <= i2 as int <= NUM_DISK_PAGES as int
-    invariant dis == IdxsSeq(i2 as nat, NUM_DISK_PAGES as int);
-    invariant |cache_idx_of_page_array| == NUM_DISK_PAGES as int
-    invariant forall j | i2 as int <= j < NUM_DISK_PAGES as int :: j !in cache_idx_of_page_array
+    while i2 < config.num_disk_pages
+    invariant 0 <= i2 as int <= config.num_disk_pages as int
+    invariant dis == IdxsSeq(i2 as nat, CacheSSM.MAX_DISK_PAGES)
+    invariant |cache_idx_of_page_array| == config.num_disk_pages as int
+    invariant forall j | i2 as int <= j < config.num_disk_pages as int :: j !in cache_idx_of_page_array
     invariant forall j | 0 <= j < i2 as int :: j in cache_idx_of_page_array
-        && atomic_index_lookup_inv(cache_idx_of_page_array[j], j)
-    decreases NUM_DISK_PAGES as int - i2 as int
+        && atomic_index_lookup_inv(cache_idx_of_page_array[j], j, config)
+    decreases config.num_disk_pages as int - i2 as int
     {
       glinear var di;
-      di, dis := pop_IdxSeq(dis, i2 as nat, NUM_DISK_PAGES as int);
+      di, dis := pop_IdxSeq(dis, i2 as nat, CacheSSM.MAX_DISK_PAGES);
       linear var ail := new_atomic(NOT_MAPPED as uint32, di,
-          (v, g) => AtomicIndexLookupImpl.state_inv(v, g, i2 as nat),
+          (v, g) => AtomicIndexLookupImpl.state_inv(v, g, i2 as nat, config),
           0);
       lseq_give_inout(inout cache_idx_of_page_array, i2, ail);
       i2 := i2 + 1;
@@ -504,34 +493,35 @@ module CacheInit(aio: AIO(CacheAIOParams, CacheIfc, CacheSSM)) {
 
     linear var io_slots;
     var iocb_base_ptr;
-    iocb_base_ptr, io_slots := init_ioslots();
+    iocb_base_ptr, io_slots := init_ioslots(config);
 
-    ghost var disk_idx_of_entry := seq(CACHE_SIZE as int, (i) requires 0 <= i < CACHE_SIZE as int =>
+    ghost var disk_idx_of_entry := seq(config.cache_size as int, (i) requires 0 <= i < config.cache_size as int =>
         status_idx_array[i].page_handle);
-    ghost var status := seq(CACHE_SIZE as int, (i) requires 0 <= i < CACHE_SIZE as int =>
+    ghost var status := seq(config.cache_size as int, (i) requires 0 <= i < config.cache_size as int =>
         status_idx_array[i].status);
     ghost var read_refcounts :=
         seq(RC_WIDTH as int, (j) requires 0 <= j < RC_WIDTH as int =>
-          seq(CACHE_SIZE as int, (i) requires 0 <= i < CACHE_SIZE as int =>
-            read_refcounts_array[rc_index(j as uint64, i as uint32) as int]));
+          seq(config.cache_size as int, (i) requires 0 <= i < config.cache_size as int =>
+            read_refcounts_array[rc_index(config, j as uint64, i as uint32) as int]));
     ghost var cache_idx_of_page :=
-        seq(NUM_DISK_PAGES as int, (i) requires 0 <= i < NUM_DISK_PAGES as int =>
+        seq(config.num_disk_pages as int, (i) requires 0 <= i < config.num_disk_pages as int =>
           cache_idx_of_page_array[i]);
 
     linear var ioctx := aio.init_ctx(
       ((iocb_ptr, iocb, wp, g) =>
-          ReadGInv(io_slots, data, disk_idx_of_entry, status, iocb_ptr, iocb, wp, g)),
+          ReadGInv(io_slots, data, disk_idx_of_entry, status, config, iocb_ptr, iocb, wp, g)),
       ((iocb_ptr, iocb, p, g) =>
-          WriteGInv(io_slots, data, disk_idx_of_entry, status, iocb_ptr, iocb, p, g)),
+          WriteGInv(io_slots, data, disk_idx_of_entry, status, config, iocb_ptr, iocb, p, g)),
       ((iocb_ptr, iocb, x, p, g) =>
-          ReadvGInv(io_slots, data, disk_idx_of_entry, status, iocb_ptr, iocb, x, p, g)),
+          ReadvGInv(io_slots, data, disk_idx_of_entry, status, config, iocb_ptr, iocb, x, p, g)),
       ((iocb_ptr, iocb, x, p, g) =>
-          WritevGInv(io_slots, data, disk_idx_of_entry, status, iocb_ptr, iocb, x, p, g))
+          WritevGInv(io_slots, data, disk_idx_of_entry, status, config, iocb_ptr, iocb, x, p, g))
     );
 
-    linear var batch_busy := init_batch_busy();
+    linear var batch_busy := init_batch_busy(config);
 
     c := Cache(
+        config,
         data_base_ptr,
         iocb_base_ptr,
         read_refcounts_array,
@@ -549,7 +539,7 @@ module CacheInit(aio: AIO(CacheAIOParams, CacheIfc, CacheSSM)) {
         ioctx,
         counter_loc);
 
-    forall i | 0 <= i < CACHE_SIZE as int
+    forall i | 0 <= i < config.cache_size as int
     ensures data[i].aligned(PageSize as int)
     {
       assert has_single(data_pta_full, PageSize as int, data_pta_seq_copy, i as int);
@@ -558,19 +548,19 @@ module CacheInit(aio: AIO(CacheAIOParams, CacheIfc, CacheSSM)) {
       assert data[i].aligned(PageSize as int);
     }
 
-    forall j, i | 0 <= j < RC_WIDTH as int && 0 <= i < CACHE_SIZE as int
+    forall j, i | 0 <= j < RC_WIDTH as int && 0 <= i < config.cache_size as int
     ensures read_refcounts[j][i].inv(j)
     ensures read_refcounts[j][i].rwlock_loc == status[i].rwlock_loc
     {
-      refcount_i_inv_i_get(read_refcounts_array, status_idx_array, counter_loc, CACHE_SIZE, i, j);
+      refcount_i_inv_i_get(config, read_refcounts_array, status_idx_array, counter_loc, config.cache_size as int, i, j);
       reveal_refcount_i_inv();
-      var rci := rc_index(j as uint64, i as uint32) as int;
+      var rci := rc_index(config, j as uint64, i as uint32) as int;
       assert read_refcounts[j][i] == 
           read_refcounts_array[rci];
       assert read_refcounts_array[rci].inv(j);
     }
 
-    ghost var i0 := CACHE_SIZE as int - 1;
+    ghost var i0 := config.cache_size as int - 1;
     assert i0 in data_pta_seq_copy;
     assert data_base_ptr.as_nat() == data_pta_full.ptr.as_nat();
     assert 0 <= data_pta_full.ptr.as_nat() + i0 * PageSize as int < 0x1_0000_0000_0000_0000
@@ -579,28 +569,28 @@ module CacheInit(aio: AIO(CacheAIOParams, CacheIfc, CacheSSM)) {
       sizeof_int_types();
     }
 
-    forall i | 0 <= i < RC_WIDTH as int * CACHE_SIZE as int
+    forall i | 0 <= i < RC_WIDTH as int * config.cache_size as int
     ensures lseq_has(read_refcounts_array)[i]
     {
-      var j1, i1 := inverse_rc_index(i);
-      var rci := rc_index(j1 as uint64, i1 as uint32) as int;
+      var j1, i1 := inverse_rc_index(config, i);
+      var rci := rc_index(config, j1 as uint64, i1 as uint32) as int;
       assert i == rci;
-      refcount_i_inv_i_get(read_refcounts_array, status_idx_array, counter_loc, CACHE_SIZE, i1, j1);
+      refcount_i_inv_i_get(config, read_refcounts_array, status_idx_array, counter_loc, config.cache_size as int, i1, j1);
       reveal_refcount_i_inv();
       assert lseq_has(read_refcounts_array)[rci];
     }
 
     forall j, i {:trigger c.read_refcounts[j][i]}
-        | 0 <= j < RC_WIDTH as int && 0 <= i < CACHE_SIZE as int
+        | 0 <= j < RC_WIDTH as int && 0 <= i < config.cache_size as int
     ensures c.read_refcounts[j][i].inv(j)
     ensures c.read_refcounts[j][i].rwlock_loc == c.status[i].rwlock_loc
     ensures c.read_refcounts[j][i].counter_loc == counter_loc
     {
-      refcount_i_inv_i_get(read_refcounts_array, status_idx_array, counter_loc, CACHE_SIZE, i, j);
+      refcount_i_inv_i_get(config, read_refcounts_array, status_idx_array, counter_loc, config.cache_size as int, i, j);
       reveal_refcount_i_inv();
     }
 
-    forall i | 0 <= i < CACHE_SIZE as int
+    forall i | 0 <= i < config.cache_size as int
     ensures c.data[i] == ptr_add(c.data_base_ptr, (PageSize as int * i) as uint64)
     {
       assert has_single(data_pta_full, PageSize as int, data_pta_seq_copy, i);
@@ -611,9 +601,10 @@ module CacheInit(aio: AIO(CacheAIOParams, CacheIfc, CacheSSM)) {
     assert c.Inv();
   }
 
-  method init_thread_local_state(t: uint64)
+  method init_thread_local_state(ghost cache: Cache, t: uint64)
   returns (linear l: LocalState)
-  ensures l.WF()
+  requires cache.Inv()
+  ensures l.WF(cache.config)
   {
     l := LocalState(t % RC_WIDTH_64(), 0xffff_ffff_ffff_ffff, 0);
   }
