concurrency/scache/Constants.i.dfy
@@ -1,39 +1,274 @@
 include "../../lib/Lang/NativeTypes.s.dfy"
+include "../Math/Math.i.dfy"
 
 module Constants {
   import opened NativeTypes
+  import NonlinearLemmas
+  import Math
+
+  function method PLATFORM_CACHELINE_SIZE_64(): uint64 { 64 }
+  function method ENTRIES_PER_BATCH_32(): uint32 { 64 }
+
+  datatype PreConfig = PreConfig(
+    cache_size: uint32,
+    num_disk_pages: uint64,
+    pages_per_extent: uint64
+  )
+  {
+    predicate WF() {
+      && cache_size as int % PLATFORM_CACHELINE_SIZE_64() as int == 0
+      && cache_size as int % ENTRIES_PER_BATCH_32() as int == 0
+      && cache_size as int > 0
+      && cache_size as int < 0x4000_0000
+      && 0 < num_disk_pages as int < 0x1_0000_0000_0000
+      && pages_per_extent != 0
+      && pages_per_extent <= 0x1_0000
+    }
+  }
+
+  datatype Config = Config(
+    cache_size: uint32,
+    num_disk_pages: uint64,
+
+    pages_per_extent: uint64,
+
+    batch_capacity: uint64,
+    cacheline_capacity: uint64
+  )
+  {
+    predicate WF() {
+      && cacheline_capacity != 0
+      && pages_per_extent != 0
+      && pages_per_extent <= 0x1_0000
+      && cache_size as int == cacheline_capacity as int * PLATFORM_CACHELINE_SIZE_64() as int
+      && cache_size as int == batch_capacity as int * ENTRIES_PER_BATCH_32() as int
+      && cache_size as int * RC_WIDTH < 0x1_0000_0000
+      && num_disk_pages as int * 4096 < 0x1000_0000_0000_0000
+      && 0 < num_disk_pages as int
+    }
+  }
+
+  method fromPreConfig(pre: PreConfig) returns (config: Config)
+  requires pre.WF()
+  ensures config.WF()
+  {
+    config := Config(pre.cache_size, pre.num_disk_pages, pre.pages_per_extent,
+        pre.cache_size as uint64 / ENTRIES_PER_BATCH_32() as uint64,
+        pre.cache_size as uint64 / PLATFORM_CACHELINE_SIZE_64());
+  }
 
   ghost const RC_WIDTH := 4;
-  //const CACHE_SIZE := 1048576;
-  //const NUM_DISK_PAGES := 536870912;
-
-  // Using smaller constants to make small experiments faster
-  ghost const CACHE_SIZE := 131072;
-  ghost const NUM_DISK_PAGES := 7864320;
 
   ghost const CHUNK_SIZE := 64;
-  ghost const NUM_CHUNKS := CACHE_SIZE / 64;
   ghost const CLEAN_AHEAD := 512;
 
   ghost const NUM_IO_SLOTS := 256;
   ghost const AIO_HAND_BATCH_SIZE := 32;
 
-  ghost const PAGES_PER_EXTENT := 32;
-
-  function method CACHE_SIZE_64(): uint64 { 131072 }
-  function method NUM_DISK_PAGES_64(): uint64 { 7864320 }
+  function method CHUNK_SIZE_32(): uint32 { 64 }
   function method AIO_HAND_BATCH_SIZE_64(): uint64 { 32 }
   function method NUM_IO_SLOTS_64(): uint64 { 256 }
-  function method PAGES_PER_EXTENT_64(): uint64 { 32 }
-  function method CHUNK_SIZE_32(): uint32 { 64 }
   function method DEFAULT_MAX_IO_EVENTS_64(): uint64 { 32 }
   function method RC_WIDTH_64(): uint64 { 4 }
-  function method NUM_CHUNKS_64(): uint64 { CACHE_SIZE_64() / 64 }
   function method CLEAN_AHEAD_64(): uint64 { 512 }
 
-  function method PLATFORM_CACHELINE_SIZE_64(): uint64 { 64 }
+  function method {:opaque} rc_index(config: Config, j: uint64, i: uint32) : (k: uint64)
+  requires config.WF()
+  requires 0 <= j as int < RC_WIDTH as int
+  requires 0 <= i as int < config.cache_size as int
+  ensures 0 <= k as int < RC_WIDTH as int * config.cache_size as int
+  {
+    NonlinearLemmas.mod_bound(i as int, config.cacheline_capacity as int);
+    Math.div_bound(i as int, config.cacheline_capacity as int);
+    Math.mod_div_transpose_bound(i as int, config.cacheline_capacity as int,
+        PLATFORM_CACHELINE_SIZE_64() as int);
+    NonlinearLemmas.mul_le_left(j as int, config.cache_size as int, RC_WIDTH as int - 1);
 
-  function CACHELINE_CAPACITY() : int
-  ensures CACHELINE_CAPACITY() == CACHE_SIZE / PLATFORM_CACHELINE_SIZE_64() as int
-  { 2048 }
+    //var cacheline_capacity := config.cache_size / PLATFORM_CACHELINE_SIZE_64() as uint32;
+    //assert cacheline_capacity as int == CACHELINE_CAPACITY();
+    var rc_number := (i % config.cacheline_capacity as uint32) * PLATFORM_CACHELINE_SIZE_64() as uint32
+        + (i / config.cacheline_capacity as uint32);
+    (j as uint32 * config.cache_size + rc_number) as uint64
+  }
+
+  lemma inverse_rc_index(config: Config, k: int)
+  returns (j: int, i: int)
+  requires config.WF()
+  requires 0 <= k as int < RC_WIDTH as int * config.cache_size as int
+  ensures 0 <= j as int < RC_WIDTH as int
+  ensures 0 <= i as int < config.cache_size as int
+  ensures k == rc_index(config, j as uint64, i as uint32) as int
+  {
+    j := k / config.cache_size as int;
+    var rc_number := k % config.cache_size as int;
+
+    var cacheline_capacity: int := (config.cache_size as int / PLATFORM_CACHELINE_SIZE_64() as int) as int;
+    //assert cacheline_capacity as int == CACHELINE_CAPACITY();
+
+    i := (rc_number % (PLATFORM_CACHELINE_SIZE_64() as int)) * cacheline_capacity
+        + (rc_number / (PLATFORM_CACHELINE_SIZE_64() as int));
+
+    var rc_number2 := (i % cacheline_capacity) * (PLATFORM_CACHELINE_SIZE_64() as int)
+        + (i / cacheline_capacity);
+
+    if j >= RC_WIDTH as int {
+      NonlinearLemmas.div_mul_plus_mod(k, config.cache_size as int);
+      NonlinearLemmas.mod_bound(k, config.cache_size as int);
+      NonlinearLemmas.mul_le_left(RC_WIDTH as int, k / config.cache_size as int,
+          config.cache_size as int);
+      assert false;
+    }
+    assert 0 <= j by {
+      Math.div_bound(k, config.cache_size as int);
+    }
+
+    if i / cacheline_capacity >= PLATFORM_CACHELINE_SIZE_64() as int {
+      NonlinearLemmas.div_mul_plus_mod(i, cacheline_capacity);
+      NonlinearLemmas.mod_bound(i, cacheline_capacity);
+      NonlinearLemmas.mul_le_left(PLATFORM_CACHELINE_SIZE_64() as int,
+          i / cacheline_capacity, cacheline_capacity);
+    }
+
+    NonlinearLemmas.mod_bound(rc_number, PLATFORM_CACHELINE_SIZE_64() as int);
+    Math.div_bound(rc_number, PLATFORM_CACHELINE_SIZE_64() as int);
+    Math.mod_div_transpose_bound(rc_number,
+        PLATFORM_CACHELINE_SIZE_64() as int,
+        config.cacheline_capacity as int);
+
+    NonlinearLemmas.mod_bound(i as int, config.cacheline_capacity as int);
+    Math.div_bound(i as int, config.cacheline_capacity as int);
+    Math.mod_div_transpose_bound(i as int, config.cacheline_capacity as int,
+        PLATFORM_CACHELINE_SIZE_64() as int);
+
+    NonlinearLemmas.mul_le_left(j as int, config.cache_size as int, RC_WIDTH as int - 1);
+
+    calc {
+      rc_number2 % (PLATFORM_CACHELINE_SIZE_64() as int);
+      (i / cacheline_capacity);
+      {
+        Math.lemma_div_multiples_vanish_fancy(
+            (rc_number % (PLATFORM_CACHELINE_SIZE_64() as int)),
+            (rc_number / (PLATFORM_CACHELINE_SIZE_64() as int)),
+            cacheline_capacity);
+        NonlinearLemmas.mul_comm(
+            (rc_number % (PLATFORM_CACHELINE_SIZE_64() as int)),
+            cacheline_capacity);
+      }
+      rc_number % (PLATFORM_CACHELINE_SIZE_64() as int);
+    }
+
+    calc {
+      rc_number2 / (PLATFORM_CACHELINE_SIZE_64() as int);
+      {
+        /*
+        Math.lemma_div_multiples_vanish_fancy(
+            i % cacheline_capacity, i / cacheline_capacity,
+            PLATFORM_CACHELINE_SIZE_64() as int);
+        NonlinearLemmas.mul_comm(i % cacheline_capacity,
+            PLATFORM_CACHELINE_SIZE_64() as int);
+            */
+      }
+      (i % cacheline_capacity);
+      {
+        Math.abc_mod(
+          (rc_number % (PLATFORM_CACHELINE_SIZE_64() as int)),
+          cacheline_capacity,
+          (rc_number / (PLATFORM_CACHELINE_SIZE_64() as int)));
+      }
+      rc_number / (PLATFORM_CACHELINE_SIZE_64() as int);
+    }
+
+    calc {
+      k;
+      {
+        NonlinearLemmas.div_mul_plus_mod(k, config.cache_size as int);
+      }
+      (k / config.cache_size as int) * config.cache_size as int + k % config.cache_size as int;
+      {
+        assert rc_number == rc_number2;
+        reveal_rc_index();
+      }
+      rc_index(config, j as uint64, i as uint32) as int;
+    }
+  }
+
+  lemma rc_index_inj(config: Config, j1: int, i1: int, j2: int, i2: int)
+  requires config.WF()
+  requires 0 <= j1 as int < RC_WIDTH as int
+  requires 0 <= i1 as int < config.cache_size as int
+  requires 0 <= j2 as int < RC_WIDTH as int
+  requires 0 <= i2 as int < config.cache_size as int
+  ensures rc_index(config, j1 as uint64, i1 as uint32)
+      == rc_index(config, j2 as uint64, i2 as uint32) ==> i1 == i2 && j1 == j2
+  {
+    if rc_index(config, j1 as uint64, i1 as uint32)
+      == rc_index(config, j2 as uint64, i2 as uint32)
+    {
+      reveal_rc_index();
+
+      var rc_number1 := (i1 % config.cacheline_capacity as int) * PLATFORM_CACHELINE_SIZE_64() as int
+          + (i1 / config.cacheline_capacity as int);
+
+      Math.mod_div_transpose_bound(i1 as int, config.cacheline_capacity as int,
+          PLATFORM_CACHELINE_SIZE_64() as int);
+
+      var rc_number2 := (i2 % config.cacheline_capacity as int) * PLATFORM_CACHELINE_SIZE_64() as int
+          + (i2 / config.cacheline_capacity as int);
+
+      Math.mod_div_transpose_bound(i2 as int, config.cacheline_capacity as int,
+          PLATFORM_CACHELINE_SIZE_64() as int);
+
+      var k := rc_index(config, j1 as uint64, i1 as uint32) as int;
+
+      calc {
+        rc_number1;
+        { Math.abc_mod(j1, config.cache_size as int, rc_number1); }
+        k % config.cache_size as int;
+        { Math.abc_mod(j2, config.cache_size as int, rc_number2); }
+        rc_number2;
+      }
+
+      Math.ab_div_lt(PLATFORM_CACHELINE_SIZE_64() as int,
+          config.cacheline_capacity as int, i1);
+      Math.ab_div_lt(PLATFORM_CACHELINE_SIZE_64() as int,
+          config.cacheline_capacity as int, i2);
+
+      calc {
+        i1 / config.cacheline_capacity as int;
+        {
+          Math.abc_mod(i1 % config.cacheline_capacity as int,
+            PLATFORM_CACHELINE_SIZE_64() as int,
+            i1 / config.cacheline_capacity as int);
+        }
+        rc_number1 % PLATFORM_CACHELINE_SIZE_64() as int;
+        rc_number2 % PLATFORM_CACHELINE_SIZE_64() as int;
+        i2 / config.cacheline_capacity as int;
+      }
+
+      calc {
+        i1 % config.cacheline_capacity as int;
+        rc_number1 / PLATFORM_CACHELINE_SIZE_64() as int;
+        rc_number2 / PLATFORM_CACHELINE_SIZE_64() as int;
+        i2 % config.cacheline_capacity as int;
+      }
+
+      NonlinearLemmas.div_mul_plus_mod(i1, config.cacheline_capacity as int);
+      NonlinearLemmas.div_mul_plus_mod(i2, config.cacheline_capacity as int);
+
+      calc {
+        j1;
+        {
+          Math.lemma_div_multiples_vanish_fancy(j1, rc_number2, config.cache_size as int);
+          NonlinearLemmas.mul_comm(j1, config.cache_size as int);
+        }
+        k / config.cache_size as int;
+        {
+          Math.lemma_div_multiples_vanish_fancy(j2, rc_number2, config.cache_size as int);
+          NonlinearLemmas.mul_comm(j2, config.cache_size as int);
+        }
+        j2;
+      }
+    }
+  }
+
 }
