concurrency/scache/cache/CacheResources.i.dfy
@@ -646,13 +646,13 @@ module CacheResources {
   glinear method split_init(glinear t: T.Token)
   returns (glinear idxs: T.Token, glinear empties: T.Token)
   requires CacheSSM.Init(t.val)
-  ensures idxs == IdxsSeq(0, NUM_DISK_PAGES as int)
-  ensures empties == EmptySeq(0, CACHE_SIZE as int)
+  ensures idxs == IdxsSeq(0, CacheSSM.MAX_DISK_PAGES as int)
+  ensures empties == EmptySeq(0, CacheSSM.MAX_CACHE_SIZE as int)
   {
     reveal_EmptyRange();
     reveal_IdxsRange();
     idxs, empties := TU.split2(t,
-        IdxsSeq(0, NUM_DISK_PAGES as int).val,
-        EmptySeq(0, CACHE_SIZE as int).val);
+        IdxsSeq(0, CacheSSM.MAX_DISK_PAGES as int).val,
+        EmptySeq(0, CacheSSM.MAX_CACHE_SIZE as int).val);
   }
 }
